\documentclass{report}

\usepackage{amsmath}
\usepackage{amsfonts}
\DeclareMathOperator*{\argmax}{arg\,max}

\begin{document}
   \textbf{word2vec gradients} \quad Charlie Colley \quad 9/29/17\\
   
   
   
   $ \sigma(x) = \frac{1}{1 + e^{x}} $
   \[\frac{\partial \sigma}{\partial x}(x) 
     =  \frac{\partial}{\partial x}(\frac{e^x}{1+e^x}) 
     =  \frac{(1 + e^x)e^x - e^x(e^x)}{(1 + e^x)^2} 
     = (\frac{e^x}{1+ e^x})(\frac{1 - e^x + e^x}{(1 + e^x)}) \]
     \[
     = \sigma(x)(\frac{1+e^x}{1+e^x} -\frac{e^x}{(1+e^x)})
     = \sigma(x)(1 - \sigma(x))
   \]
   Thus  $\frac{\partial \sigma(x)}{\partial x}(x) =
           \sigma(x)(1 - \sigma(x))$.
           
\vspace{10 mm}
   Objective function:\\
   $ \displaystyle\argmax_{V_c, V_w} 
     = \displaystyle\Sigma_{(w,c) \in D} 
     \log(\sigma(\langle v_c, v_w\rangle))  +\displaystyle\Sigma_{(w,c)v\in D'} 
         \log(\sigma(-\langle v_c, v_w \rangle)) $

   \[
      \nabla_{v_c} (\langle v_c, v_w \rangle)_k = \frac{\partial}{\partial (v_c)_k}\displaystyle \sum_{i}(v_c)_i(v_w)_i = \frac{\partial}{\partial (v_c)_k}(\displaystyle \sum_{i \neq k}(v_c)_i(v_w)_i + (v_c)_k(v_w)_k) = (v_w)_k
   \]
   by symmetry, the gradient $\nabla_{v_w} \langle v_c, v_w \rangle $ is $ v_c $.
   Let $ B \in \mathbb{R}^{n \times m}$.
     
    \[ \nabla_{B} (\langle v_c, v_w \rangle_{B})_{kl} = \frac{\partial}{\partial B_{kl}}\displaystyle \sum_{ij}B_{ij}(v_c)_i(v_w)_i = \]
    \[\frac{\partial}{\partial B_{kl}}(\displaystyle \sum_{i,j \neq k}(v_c)_i(v_w)_i + B_{kl}(v_c)_k(v_w)_l) = (v_c)_l(v_w)_k = (v_c \otimes v_w)_{kl}\]
    
    Then the gradient of $ \log(\sigma(\langle v_c, v_w \rangle )) $ with respect to $ v_c $ is 
    \[
      \frac{\partial}{\partial (v_c)_k}(\log(\sigma(\langle v_c, v_w \rangle)))
      = (\frac{1}{\sigma(\langle v_c, v_w \rangle)})(\sigma(\langle v_c, v_w \rangle)(1 - \sigma(\langle v_c, v_w \rangle)))(v_w)_k 
    \]
    \[
      = (1 - \sigma(\langle v_c, v_w \rangle)))(v_w)_k 
    \]
    again by symmetry we can show that the gradient with respect to $ v_w $ is similarly $ \nabla_{v_w}(log(\sigma(\langle v_c, v_w \rangle))) = (1 - \sigma(\langle v_c, v_w \rangle))v_c $
    
    

   
   \newpage
   Let $ P \in \mathbb{R}^{n \times n} $ and $ U, V \in \mathbb{R}^{n \times d} $ and let $ f = \|P - UV^T\|_F^2 $
   \begin{align*}
     (\nabla_U f)_{ij} =& \frac{\partial}{\partial U_{ij}}\|P - UV^T\|_F^2 = 
     \frac{\partial}{\partial U_{ij}} (\displaystyle \sum_{i_1,i_2 =1}^n(P_{i_1,i_2} 
                     - \displaystyle\sum_{i_3}^d U_{i_1,i_3}V^T_{i_3,i_2})^2)  \\
       =& \frac{\partial}{\partial U_{ij}} (\lbrack \displaystyle \sum_{i_1 \neq i,i_2 =1}^n(P_{i_1,i_2} 
       - \displaystyle\sum_{i_3}^d U_{i_1,i_3}V^T_{i_3,i_2})^2 \rbrack + (P_{i,i_2} 
       - \displaystyle\sum_{i_3}^d U_{i,i_3}V^T_{i_3,i_2})^2)\\
       =& \frac{\partial}{\partial U_{ij}}\displaystyle\sum_{i_2}^n(P_{i,i_2} 
       - \displaystyle\sum_{i_3}^d U_{i,i_3}V^T_{i_3,i_2})^2 \\
       =& \displaystyle\sum_{i_2}^n2(P_{i,i_2} 
       - \displaystyle\sum_{i_3}^d U_{i,i_3}V^T_{i_3,i_2})\frac{\partial}{\partial U_{ij}}(P_{i,i_2} 
       - \displaystyle\sum_{i_3}^d U_{i,i_3}V^T_{i_3,i_2}) \\
       =& \displaystyle\sum_{i_2} 2(P_{i,i_2} 
       - \displaystyle\sum_{i_3}^d U_{i,i_3}V^T_{i_3,i_2})(V^T_{j,i_2}) \\
       =& \displaystyle\sum_{i_2} 2(P_{i,i_2} 
       - (UV^T)_{i,i_2})(V_{i_2,j}) = 2(PV - UV^TV)_{ij}
   \end{align*}
 
  \[
    (\nabla_Vf)_{ij} 
    = \frac{\partial}{\partial V_{ij}}\|P - UV^T\|^2_F = \frac{\partial}{\partial V_{ij}}\|P^T - VU^T\|^2_F
  \]
   	Now note that by the generality of the last gradient computation we can show that $ \nabla_Vf = 2(P^TU - VU^TU) $.
   	
   	Consider the function $ g = \lambda\|U\|_F^2 $ for $ \lambda \in \mathbb{R} $, then the gradient with respect to $ U $ is 
   	
   	\[ 
   	 (\nabla_{U}g)_{ij} 
   	   = \lambda
   	     \frac{\partial}{\partial U_{ij}}(\sum_{i_1,i_2 = 1}^{n,d}U^2_{i_1,i_2})
   	   = \lambda \frac{\partial}{\partial U_{ij}}
   	     (\lbrack \sum_{i_1 \neq i,i_2 \neq j}^{n,d}U^2_{i_1,i_2}\rbrack + U_{ij}^2) = 2\lambda U_{ij}
   	\]
   	
   	\newpage
   	Let $ P \in \mathbb{R}^{n \times n} $, $ U \in \mathbb{R}^{n \times d} $, and $B \in \mathbb{R}^{d \times d} $. Consider the function $ f: \mathbb{R}^{n \times n} \times \mathbb{R}^{n \times d} \times \mathbb{R}^{n \times n} \mapsto \mathbb{R} $ such that 
   	\[ 
   	  f(P,U,B) = \|P - UBB^TU^T\|_F^2
   	\]
   	Letting $ C = BB^T $
   	\begin{align*}
   		 (\nabla_{U}f)_{ij}
   		 &= \frac{\partial}{\partial U_{ij}}\|P - UBB^TU^T\|_F^2 
   		  = \frac{\partial}{\partial U_{ij}}\|P - UCU^T\|_F^2 
   		  = \frac{\partial}{\partial U_{ij}}\displaystyle \sum_{i_1,i_2}^{n,n} (P_{i_1,i_2} -  (UCU^T)_{i_1,i_2})^2 \\
   		 &= \frac{\partial}{\partial U_{ij}} \sum_{i_1,i_2}^{n,n} (P_{i_1,i_2} -    \sum_{i_3}^{d}(U_{i_1,i_3}(CU^T)_{i_3,i_2})^2 
   		  = \frac{\partial}{\partial U_{ij}} \sum_{i_1,i_2}^{n,n} (P_{i_1,i_2} - \sum_{i_3,i_4}^{d,d}U_{i_1,i_3}C_{i_3,i_4}U^T_{i_4,i_2})^2 \\
   		 &= \frac{\partial}{\partial U_{ij}} (\big[\sum_{\substack{i_1,i_2 \\ (i_1,i_2) \neq (i,j)}}^{n,n} (P_{i_1,i_2} - \sum_{i_3,i_4}^{d,d}U_{i_1,i_3}C_{i_3,i_4}U^T_{i_4,i_2})^2\big] + (P_{i,j} - \sum_{i_3,i_4}^{d,d}U_{i,i_3}C_{i_3,i_4}U^T_{i_4,j})^2) \\
   		 &= \frac{\partial}{\partial U_{ij}}((P_{i,j} - \sum_{i_3,i_4}^{d,d}U_{i,i_3}C_{i_3,i_4}U^T_{i_4,j})^2) \\
   		 &= 2(P_{i,j} - \sum_{i_3,i_4}^{d,d}U_{i,i_3}C_{i_3,i_4}U^T_{i_4,j})\frac{\partial}{\partial U_{ij}}(P_{i,j} - \sum_{i_3,i_4}^{d,d}U_{i,i_3}C_{i_3,i_4}U^T_{i_4,j}) \\
   		 &= 2(P_{i,j} - \sum_{i_3,i_4}^{d,d}U_{i,i_3}C_{i_3,i_4}U^T_{i_4,j})\frac{\partial}{\partial U_{ij}}(-\sum_{i_3,i_4}^{d,d}U_{i,i_3}C_{i_3,i_4}U^T_{i_4,j}) \\
   		 &= 2(P_{i,j} - \sum_{i_3,i_4}^{d,d}U_{i,i_3}C_{i_3,i_4}U^T_{i_4,j})\frac{-\partial}{\partial U_{ij}}(\big[\sum_{\substack{i_3,i_4\\ i_3 \neq j}}^{d,d}U_{i,i_3}C_{i_3,i_4}U^T_{i_4,j}\big] + U_{i,j}\sum_{i_4}^dC_{j,i_4}U^T_{i_4,j}) \\
   		 &=2(P_{i,j} - \sum_{i_3,i_4}^{d,d}U_{i,i_3}C_{i_3,i_4}U^T_{i_4,j})\frac{-\partial}{\partial U_{ij}}(U_{i,j}\sum_{i_4}^dC_{j,i_4}U^T_{i_4,j}) \\
   		 &= -2(P_{i,j} - \sum_{i_3,i_4}^{d,d}U_{i,i_3}C_{i_3,i_4}U^T_{i_4,j})(\sum_{i_4}^dC_{j,i_4}U^T_{i_4,j}) \\
   		 &= -2(P_{i,j} - (UCU^T)_{i,j})(CU^T)_{j,j}
   		 = -2(P_{i,j} - (UBB^TU^T)_{i,j})(BB^TU^T)_{j,j}   	
   		 \end{align*}
\end{document}